formatting

cedar-lean/Cedar/Thm/Validation/Validator.lean
@@ -10,227 +10,252 @@ open Cedar.Data
 open Cedar.Spec
 open Cedar.Validation
 
--- for a single expression, evaluates to a boolean value (or appropriate error)
+/-- for a single expression, evaluates to a boolean value (or appropriate error) -/
 def OneEvaluatesCorrectly (expr : Expr) (request : Request) (entities : Entities) : Prop :=
-∃ (b : Bool), EvaluatesTo expr request entities b
+  ∃ (b : Bool), EvaluatesTo expr request entities b
 
--- every policy as an expression evaluates to a boolean value or appropriate error
+/-- every policy as an expression evaluates to a boolean value or appropriate error -/
 def AllEvaluateCorrectly (policies : Policies) (request : Request) (entities : Entities) : Prop :=
-∀ policy : Policy, policy ∈ policies → OneEvaluatesCorrectly policy.toExpr request entities
+  ∀ policy : Policy, policy ∈ policies → OneEvaluatesCorrectly policy.toExpr request entities
+
+def RequestAndEntitiesMatchSchema (schema : Schema) (request : Request) (entities : Entities) :Prop :=
+  ∀ env ∈ schema.toEnvironments,
+  RequestAndEntitiesMatchEnvironment env request entities
 
 def EvaluatesSubst (expr : Expr) (request : Request) (entities : Entities) : Prop :=
-evaluate (substituteAction request.action expr) request entities = evaluate expr request entities
+  evaluate (substituteAction request.action expr) request entities = evaluate expr request entities
 
 theorem evaluates_subst_ite {i t e : Expr} {request : Request} {entities : Entities}
 (ih₁ : EvaluatesSubst i request entities)
 (ih₂ : EvaluatesSubst t request entities)
 (ih₃ : EvaluatesSubst e request entities) :
-evaluate (substituteAction request.action (Expr.ite i t e)) request entities =
-evaluate (Expr.ite i t e) request entities := by
-simp [EvaluatesSubst, substituteAction, mapOnVars] at *
-simp [evaluate, ih₁, ih₂, ih₃]
+  evaluate (substituteAction request.action (Expr.ite i t e)) request entities =
+  evaluate (Expr.ite i t e) request entities
+:= by
+  simp only [EvaluatesSubst, substituteAction, mapOnVars] at *
+  simp only [evaluate, ih₁, ih₂, ih₃]
 
 theorem evaluates_subst_getAttr {e : Expr} {attr : Attr} {request : Request} {entities : Entities}
 (ih₁ : EvaluatesSubst e request entities) :
-evaluate (substituteAction request.action (Expr.getAttr e attr)) request entities =
-evaluate (Expr.getAttr e attr) request entities := by
-simp [EvaluatesSubst] at ih₁
-simp [substituteAction, mapOnVars] at *
-simp [evaluate, ih₁]
+  evaluate (substituteAction request.action (Expr.getAttr e attr)) request entities =
+  evaluate (Expr.getAttr e attr) request entities
+:= by
+  simp only [EvaluatesSubst] at ih₁
+  simp only [substituteAction, mapOnVars] at *
+  simp only [evaluate, ih₁]
 
 theorem evaluates_subst_hasAttr {e : Expr} {attr : Attr} {request : Request} {entities : Entities}
 (ih₁ : EvaluatesSubst e request entities) :
-evaluate (substituteAction request.action (Expr.hasAttr e attr)) request entities =
-evaluate (Expr.hasAttr e attr) request entities := by
-simp [EvaluatesSubst] at ih₁
-simp [substituteAction, mapOnVars] at *
-simp [evaluate, ih₁]
+  evaluate (substituteAction request.action (Expr.hasAttr e attr)) request entities =
+  evaluate (Expr.hasAttr e attr) request entities
+:= by
+  simp only [EvaluatesSubst] at ih₁
+  simp only [substituteAction, mapOnVars] at *
+  simp only [evaluate, ih₁]
 
 theorem evaluates_subst_unaryApp {op : UnaryOp} {e : Expr} {request : Request} {entities : Entities}
 (ih₁ : EvaluatesSubst e request entities) :
-evaluate (substituteAction request.action (Expr.unaryApp op e)) request entities =
-evaluate (Expr.unaryApp op e) request entities := by
-simp [EvaluatesSubst] at ih₁
-simp [substituteAction, mapOnVars] at *
-simp [evaluate, ih₁]
+  evaluate (substituteAction request.action (Expr.unaryApp op e)) request entities =
+  evaluate (Expr.unaryApp op e) request entities
+:= by
+  simp only [EvaluatesSubst] at ih₁
+  simp only [substituteAction, mapOnVars] at *
+  simp only [evaluate, ih₁]
 
 theorem evaluates_subst_binaryApp {op : BinaryOp} {a b : Expr} {request : Request} {entities : Entities}
 (ih₁ : EvaluatesSubst a request entities)
 (ih₂ : EvaluatesSubst b request entities) :
-evaluate (substituteAction request.action (Expr.binaryApp op a b)) request entities =
-evaluate (Expr.binaryApp op a b) request entities := by
-simp [EvaluatesSubst] at *
-simp [substituteAction, mapOnVars] at *
-simp [evaluate, ih₁, ih₂]
+  evaluate (substituteAction request.action (Expr.binaryApp op a b)) request entities =
+  evaluate (Expr.binaryApp op a b) request entities
+:= by
+  simp only [EvaluatesSubst] at *
+  simp only [substituteAction, mapOnVars] at *
+  simp only [evaluate, ih₁, ih₂]
 
 theorem evaluates_subst_and {a b : Expr} {request : Request} {entities : Entities}
 (ih₁ : EvaluatesSubst a request entities)
 (ih₂ : EvaluatesSubst b request entities) :
-evaluate (substituteAction request.action (Expr.and a b)) request entities =
-evaluate (Expr.and a b) request entities := by
-simp [EvaluatesSubst, substituteAction, mapOnVars] at *
-simp [evaluate, ih₁, ih₂]
+  evaluate (substituteAction request.action (Expr.and a b)) request entities =
+  evaluate (Expr.and a b) request entities
+:= by
+  simp only [EvaluatesSubst, substituteAction, mapOnVars] at *
+  simp only [evaluate, ih₁, ih₂]
 
 theorem evaluates_subst_or {a b : Expr} {request : Request} {entities : Entities}
 (ih₁ : EvaluatesSubst a request entities)
 (ih₂ : EvaluatesSubst b request entities) :
-evaluate (substituteAction request.action (Expr.or a b)) request entities =
-evaluate (Expr.or a b) request entities := by
-simp [EvaluatesSubst, substituteAction, mapOnVars] at *
-simp [evaluate, ih₁, ih₂]
+  evaluate (substituteAction request.action (Expr.or a b)) request entities =
+  evaluate (Expr.or a b) request entities
+:= by
+  simp only [EvaluatesSubst, substituteAction, mapOnVars] at *
+  simp only [evaluate, ih₁, ih₂]
+
+-- theorem evaluates_subst_set_inversion {xs : List Expr} {request : Request} {entities : Entities} :
 
 theorem evaluates_subst_set {xs : List Expr} {request : Request} {entities : Entities}
 (ih₁ : ∀ xᵢ, xᵢ ∈ xs → EvaluatesSubst xᵢ request entities) :
-evaluate (substituteAction request.action (Expr.set xs)) request entities =
-evaluate (Expr.set xs) request entities := by
-simp [EvaluatesSubst] at ih₁
-sorry
+  evaluate (substituteAction request.action (Expr.set xs)) request entities =
+  evaluate (Expr.set xs) request entities
+:= by
+  simp only [EvaluatesSubst] at *
+  simp only [substituteAction, mapOnVars]
+  simp only [evaluate, ih₁]
+  simp only [List.mapM₁, List.attach_def, List.mapM_pmap_subtype (evaluate · request entities)]
+  sorry
+
+
 
 theorem evaluates_subst_record {axs : List (Attr × Expr)} {request : Request} {entities : Entities}
 (ih₁ : ∀ axᵢ, axᵢ ∈ axs → EvaluatesSubst axᵢ.snd request entities) :
-evaluate (substituteAction request.action (Expr.record axs)) request entities =
-evaluate (Expr.record axs) request entities := by
-simp [EvaluatesSubst] at ih₁
-sorry
+  evaluate (substituteAction request.action (Expr.record axs)) request entities =
+  evaluate (Expr.record axs) request entities
+:= by
+  simp only [EvaluatesSubst] at ih₁
+  sorry
 
 theorem evaluates_subst_call {xfn : ExtFun} {xs : List Expr} {request : Request} {entities : Entities}
 (ih₁ : ∀ xᵢ, xᵢ ∈ xs → EvaluatesSubst xᵢ request entities) :
-evaluate (substituteAction request.action (Expr.call xfn xs)) request entities =
-evaluate (Expr.call xfn xs) request entities := by
-simp [EvaluatesSubst] at ih₁
-sorry
+  evaluate (substituteAction request.action (Expr.call xfn xs)) request entities =
+  evaluate (Expr.call xfn xs) request entities
+:= by
+  simp only [EvaluatesSubst] at ih₁
+  sorry
 
 theorem evaluates_subst (expr : Expr) (request : Request) (entities : Entities) :
-evaluate (substituteAction request.action expr) request entities =
-evaluate expr request entities := by
-cases h₀ : expr with
-| lit p => simp [substituteAction, mapOnVars]
-| var vr =>
-  cases h₁ : vr <;> simp [substituteAction, mapOnVars] <;> try assumption
-  case action => sorry
-| ite i t e =>
-  have ih₁ := evaluates_subst i request entities
-  have ih₂ := evaluates_subst t request entities
-  have ih₃ := evaluates_subst e request entities
-  exact @evaluates_subst_ite i t e request entities ih₁ ih₂ ih₃
-| and a b =>
-  have ih₁ := evaluates_subst a request entities
-  have ih₂ := evaluates_subst b request entities
-  exact @evaluates_subst_and a b request entities ih₁ ih₂
-| or a b =>
-  have ih₁ := evaluates_subst a request entities
-  have ih₂ := evaluates_subst b request entities
-  exact @evaluates_subst_or a b request entities ih₁ ih₂
-| unaryApp op e =>
-  have ih₁ := evaluates_subst e request entities
-  exact @evaluates_subst_unaryApp op e request entities ih₁
-| binaryApp op a b =>
-  have ih₁ := evaluates_subst a request entities
-  have ih₂:= evaluates_subst b request entities
-  exact @evaluates_subst_binaryApp op a b request entities ih₁ ih₂
-| getAttr x attr =>
-  have ih₁ := evaluates_subst x request entities
-  exact @evaluates_subst_getAttr x attr request entities ih₁
-| hasAttr x attr =>
-  have ih₁ := evaluates_subst x request entities
-  exact @evaluates_subst_hasAttr x attr request entities ih₁
-| set xs =>
-  have ih : ∀ xᵢ, xᵢ ∈ xs → EvaluatesSubst xᵢ request entities := by
-    intro xᵢ _
-    exact @evaluates_subst xᵢ request entities
-  exact @evaluates_subst_set xs request entities ih
-| record axs =>
-  have ih : ∀ axᵢ, axᵢ ∈ axs → EvaluatesSubst axᵢ.snd request entities := by
-    intro axᵢ hᵢ
-    have _ : sizeOf axᵢ.snd < 1 + sizeOf axs := by
-      apply List.sizeOf_snd_lt_sizeOf_list hᵢ
-    exact @evaluates_subst axᵢ.snd request entities
-  exact @evaluates_subst_record axs request entities ih
-| call xfn xs =>
-  have ih : ∀ xᵢ, xᵢ ∈ xs → EvaluatesSubst xᵢ request entities := by
-    intro xᵢ _
-    exact @evaluates_subst xᵢ request entities
-  exact @evaluates_subst_call xfn xs request entities ih
+  evaluate (substituteAction request.action expr) request entities =
+  evaluate expr request entities
+:= by
+  cases h₀ : expr with
+  | lit p => simp only [substituteAction, mapOnVars]
+  | var vr =>
+    cases h₁ : vr <;> simp only [substituteAction, mapOnVars] <;> try assumption
+    case action => sorry
+  | ite i t e =>
+    have ih₁ := evaluates_subst i request entities
+    have ih₂ := evaluates_subst t request entities
+    have ih₃ := evaluates_subst e request entities
+    exact @evaluates_subst_ite i t e request entities ih₁ ih₂ ih₃
+  | and a b =>
+    have ih₁ := evaluates_subst a request entities
+    have ih₂ := evaluates_subst b request entities
+    exact @evaluates_subst_and a b request entities ih₁ ih₂
+  | or a b =>
+    have ih₁ := evaluates_subst a request entities
+    have ih₂ := evaluates_subst b request entities
+    exact @evaluates_subst_or a b request entities ih₁ ih₂
+  | unaryApp op e =>
+    have ih₁ := evaluates_subst e request entities
+    exact @evaluates_subst_unaryApp op e request entities ih₁
+  | binaryApp op a b =>
+    have ih₁ := evaluates_subst a request entities
+    have ih₂:= evaluates_subst b request entities
+    exact @evaluates_subst_binaryApp op a b request entities ih₁ ih₂
+  | getAttr x attr =>
+    have ih₁ := evaluates_subst x request entities
+    exact @evaluates_subst_getAttr x attr request entities ih₁
+  | hasAttr x attr =>
+    have ih₁ := evaluates_subst x request entities
+    exact @evaluates_subst_hasAttr x attr request entities ih₁
+  | set xs =>
+    have ih : ∀ xᵢ, xᵢ ∈ xs → EvaluatesSubst xᵢ request entities := by
+      intro xᵢ _
+      exact @evaluates_subst xᵢ request entities
+    exact @evaluates_subst_set xs request entities ih
+  | record axs =>
+    have ih : ∀ axᵢ, axᵢ ∈ axs → EvaluatesSubst axᵢ.snd request entities := by
+      intro axᵢ hᵢ
+      have _ : sizeOf axᵢ.snd < 1 + sizeOf axs := by
+        apply List.sizeOf_snd_lt_sizeOf_list hᵢ
+      exact @evaluates_subst axᵢ.snd request entities
+    exact @evaluates_subst_record axs request entities ih
+  | call xfn xs =>
+    have ih : ∀ xᵢ, xᵢ ∈ xs → EvaluatesSubst xᵢ request entities := by
+      intro xᵢ _
+      exact @evaluates_subst xᵢ request entities
+    exact @evaluates_subst_call xfn xs request entities ih
 
 theorem action_matches_env (env : Environment) (request : Request) (entities : Entities) :
-RequestAndEntitiesMatchEnvironment env request entities →
-request.action = env.reqty.action := by
-intro h₀
-simp [RequestAndEntitiesMatchEnvironment, InstanceOfRequestType] at h₀
-obtain ⟨ ⟨ _, h₁, _, _ ⟩ , _ , _⟩ := h₀
-assumption
+  RequestAndEntitiesMatchEnvironment env request entities →
+  request.action = env.reqty.action
+:= by
+  intro h₀
+  simp only [RequestAndEntitiesMatchEnvironment, InstanceOfRequestType] at h₀
+  obtain ⟨ ⟨ _, h₁, _, _ ⟩ , _ , _⟩ := h₀
+  assumption
 
 theorem typecheck_policy_is_sound (policy : Policy) (env : Environment) (t : CedarType) (request : Request) (entities : Entities) :
-RequestAndEntitiesMatchEnvironment env request entities →
-typecheckPolicy policy env = .ok t →
-∃ b : Bool, EvaluatesTo policy.toExpr request entities b := by
-intro h₁ h₂
-simp [typecheckPolicy] at h₂
-cases h₃ : typeOf (substituteAction env.reqty.action policy.toExpr) [] env <;> simp [h₃] at h₂
-split at h₂ <;> simp only [Except.ok.injEq] at h₂
-rename_i cp ht
-have hc := empty_capabilities_invariant request entities
-have ⟨_, v, h₄, h₅⟩ := type_of_is_sound hc h₁ h₃
-have ⟨b, h₆⟩ := instance_of_type_bool_is_bool v cp.fst h₅ ht
-subst h₆
-exists b
-simp [EvaluatesTo] at *
-cases h₄ with
-| inl h₁ =>
-  left
-  rw [← evaluates_subst policy.toExpr request entities]
-  rw [action_matches_env]
-  repeat assumption
-| inr h₁ => cases h₁ with
-  | inl h₂ =>
-    right
+  RequestAndEntitiesMatchEnvironment env request entities →
+  typecheckPolicy policy env = .ok t →
+  ∃ b : Bool, EvaluatesTo policy.toExpr request entities b
+:= by
+  intro h₁ h₂
+  simp only [typecheckPolicy] at h₂
+  cases h₃ : typeOf (substituteAction env.reqty.action policy.toExpr) [] env <;> simp only [List.empty_eq,
+    h₃] at h₂
+  split at h₂ <;> simp only [Except.ok.injEq] at h₂
+  rename_i cp ht
+  have hc := empty_capabilities_invariant request entities
+  have ⟨_, v, h₄, h₅⟩ := type_of_is_sound hc h₁ h₃
+  have ⟨b, h₆⟩ := instance_of_type_bool_is_bool v cp.fst h₅ ht
+  subst h₆
+  exists b
+  simp only [EvaluatesTo] at *
+  cases h₄ with
+  | inl h₁ =>
     left
     rw [← evaluates_subst policy.toExpr request entities]
     rw [action_matches_env]
     repeat assumption
-  | inr h₂ => cases h₂ with
-    | inl h₃ =>
-      right
+  | inr h₁ => cases h₁ with
+    | inl h₂ =>
       right
       left
       rw [← evaluates_subst policy.toExpr request entities]
       rw [action_matches_env]
       repeat assumption
-    | inr h₃ =>
-      right
-      right
-      right
-      rw [← evaluates_subst policy.toExpr request entities]
-      rw [action_matches_env]
-      repeat assumption
+    | inr h₂ => cases h₂ with
+      | inl h₃ =>
+        right
+        right
+        left
+        rw [← evaluates_subst policy.toExpr request entities]
+        rw [action_matches_env]
+        repeat assumption
+      | inr h₃ =>
+        right
+        right
+        right
+        rw [← evaluates_subst policy.toExpr request entities]
+        rw [action_matches_env]
+        repeat assumption
 
 theorem typecheck_policy_with_environments_is_sound (policy : Policy) (envs : List Environment) (request : Request) (entities : Entities) :
-(∀ env : Environment, env ∈ envs →
-RequestAndEntitiesMatchEnvironment env request entities) →
-typecheckPolicyWithEnvironments policy envs = .ok () →
-∃ b : Bool, EvaluatesTo policy.toExpr request entities b := by
-intro h₀ h₂
-simp [typecheckPolicyWithEnvironments] at h₂
-cases h₃ : List.mapM (typecheckPolicy policy) envs with
-| error => simp [h₃] at h₂
-| ok ts =>
-  simp [h₃] at h₂
-  cases h₄ : envs with
-  | nil =>
-    simp [h₄, pure, Except.pure] at h₃
-    subst h₃
-    simp [allFalse] at h₂
-  | cons h t =>
-      rw [List.mapM_ok_iff_forall₂] at h₃
-      have h₆ : RequestAndEntitiesMatchEnvironment h request entities := by
-        have h₇ : h ∈ envs := by simp [h₄]
-        specialize h₀ h
-        apply h₀ h₇
-      subst h₄
-      rw [List.forall₂_cons_left_iff] at h₃
-      simp only [exists_and_left] at h₃
-      obtain ⟨ b, _, _, _, _ ⟩ := h₃
-      apply typecheck_policy_is_sound policy h b
-      repeat assumption
+  (∀ env ∈ envs, RequestAndEntitiesMatchEnvironment env request entities) →
+  typecheckPolicyWithEnvironments policy envs = .ok () →
+  ∃ b : Bool, EvaluatesTo policy.toExpr request entities b
+:= by
+  intro h₀ h₂
+  simp only [typecheckPolicyWithEnvironments] at h₂
+  cases h₃ : List.mapM (typecheckPolicy policy) envs with
+  | error => simp only [h₃, Except.bind_err] at h₂
+  | ok ts =>
+    simp only [h₃, Except.bind_ok, ite_eq_right_iff, imp_false, Bool.not_eq_true] at h₂
+    cases h₄ : envs with
+    | nil =>
+      simp only [h₄, List.mapM_nil, pure, Except.pure, Except.ok.injEq] at h₃
+      subst h₃
+      simp only [allFalse, List.all_nil, Bool.true_eq_false] at h₂
+    | cons h t =>
+        rw [List.mapM_ok_iff_forall₂] at h₃
+        have h₆ : RequestAndEntitiesMatchEnvironment h request entities := by
+          have h₇ : h ∈ envs := by simp only [h₄, List.mem_cons, true_or]
+          specialize h₀ h
+          apply h₀ h₇
+        subst h₄
+        rw [List.forall₂_cons_left_iff] at h₃
+        simp only [exists_and_left] at h₃
+        obtain ⟨ b, _, _, _, _ ⟩ := h₃
+        apply typecheck_policy_is_sound policy h b
+        repeat assumption
 
 end Cedar.Thm
